HepLean/PerturbationTheory/FieldStatistics/OfFinset.lean
@@ -106,4 +106,24 @@ lemma ofFinset_union_disjoint (q : 𝓕 → FieldStatistic) (φs : List 𝓕) (a
   rw [ofFinset_union, Finset.disjoint_iff_inter_eq_empty.mp h]
   simp
 
+lemma ofFinset_filter_mul_neg (q : 𝓕 → FieldStatistic) (φs : List 𝓕) (a : Finset (Fin φs.length))
+    (p : Fin φs.length → Prop) [DecidablePred p] :
+    ofFinset q φs.get (Finset.filter p a) *
+    ofFinset q φs.get (Finset.filter (fun i => ¬ p i) a) = ofFinset q φs.get a  := by
+  rw [ofFinset_union_disjoint]
+  congr
+  exact Finset.filter_union_filter_neg_eq p a
+  exact Finset.disjoint_filter_filter_neg a a p
+
+lemma ofFinset_filter (q : 𝓕 → FieldStatistic) (φs : List 𝓕) (a : Finset (Fin φs.length))
+    (p : Fin φs.length → Prop) [DecidablePred p] :
+    ofFinset q φs.get (Finset.filter p a) = ofFinset q φs.get (Finset.filter (fun i => ¬ p i) a) *
+    ofFinset q φs.get a  := by
+  rw [← ofFinset_filter_mul_neg q φs a p]
+  conv_rhs =>
+    rhs
+    rw [mul_comm]
+  rw [← mul_assoc]
+  simp
+
 end FieldStatistic
