HepLean/PerturbationTheory/WickContraction/Join.lean
@@ -1,0 +1,978 @@
+/-
+Copyright (c) 2025 Joseph Tooby-Smith. All rights reserved.
+Released under Apache 2.0 license as described in the file LICENSE.
+Authors: Joseph Tooby-Smith
+-/
+import HepLean.PerturbationTheory.WickContraction.TimeContract
+import HepLean.PerturbationTheory.WickContraction.StaticContract
+import HepLean.PerturbationTheory.Algebras.FieldOpAlgebra.TimeContraction
+import HepLean.PerturbationTheory.WickContraction.SubContraction
+import HepLean.PerturbationTheory.WickContraction.Singleton
+
+/-!
+
+# Join of contractions
+
+-/
+
+open FieldSpecification
+variable {𝓕 : FieldSpecification}
+
+namespace WickContraction
+variable {n : ℕ} (c : WickContraction n)
+open HepLean.List
+open FieldOpAlgebra
+
+def join {φs : List 𝓕.States} (φsΛ : WickContraction φs.length)
+    (φsucΛ : WickContraction [φsΛ]ᵘᶜ.length) : WickContraction φs.length :=
+  ⟨φsΛ.1 ∪ φsucΛ.1.map (Finset.mapEmbedding uncontractedListEmd).toEmbedding, by
+    intro a ha
+    simp at ha
+    rcases ha with ha | ha
+    · exact φsΛ.2.1 a ha
+    · obtain ⟨a, ha, rfl⟩ := ha
+      rw [Finset.mapEmbedding_apply]
+      simp only [Finset.card_map]
+      exact φsucΛ.2.1 a ha, by
+    intro a ha b hb
+    simp at ha hb
+    rcases ha with ha | ha <;> rcases hb with hb | hb
+    · exact φsΛ.2.2 a ha b hb
+    · obtain ⟨b, hb, rfl⟩ := hb
+      right
+      symm
+      rw [Finset.mapEmbedding_apply]
+      apply uncontractedListEmd_finset_disjoint_left
+      exact ha
+    · obtain ⟨a, ha, rfl⟩ := ha
+      right
+      rw [Finset.mapEmbedding_apply]
+      apply uncontractedListEmd_finset_disjoint_left
+      exact hb
+    · obtain ⟨a, ha, rfl⟩ := ha
+      obtain ⟨b, hb, rfl⟩ := hb
+      simp only [EmbeddingLike.apply_eq_iff_eq]
+      rw [Finset.mapEmbedding_apply, Finset.mapEmbedding_apply]
+      rw [Finset.disjoint_map]
+      exact φsucΛ.2.2 a ha b hb⟩
+
+lemma join_congr {φs : List 𝓕.States} {φsΛ : WickContraction φs.length}
+    {φsucΛ : WickContraction [φsΛ]ᵘᶜ.length} {φsΛ' : WickContraction φs.length}
+    (h1 : φsΛ = φsΛ')  :
+    join φsΛ φsucΛ = join φsΛ' (congr (by simp [h1]) φsucΛ):= by
+  subst h1
+  rfl
+
+
+
+def joinLiftLeft {φs : List 𝓕.States} {φsΛ : WickContraction φs.length}
+    {φsucΛ : WickContraction [φsΛ]ᵘᶜ.length} : φsΛ.1 → (join φsΛ φsucΛ).1 :=
+  fun a => ⟨a, by simp [join]⟩
+
+lemma jointLiftLeft_injective {φs : List 𝓕.States} {φsΛ : WickContraction φs.length}
+    {φsucΛ : WickContraction [φsΛ]ᵘᶜ.length} :
+    Function.Injective (@joinLiftLeft _ _ φsΛ φsucΛ) := by
+  intro a b h
+  simp only [joinLiftLeft] at h
+  rw [Subtype.mk_eq_mk] at h
+  refine Subtype.eq h
+
+def joinLiftRight {φs : List 𝓕.States} {φsΛ : WickContraction φs.length}
+    {φsucΛ : WickContraction [φsΛ]ᵘᶜ.length} : φsucΛ.1 → (join φsΛ φsucΛ).1 :=
+  fun a => ⟨a.1.map uncontractedListEmd, by
+    simp only [join, Finset.le_eq_subset, Finset.mem_union, Finset.mem_map,
+      RelEmbedding.coe_toEmbedding]
+    right
+    use a.1
+    simp only [Finset.coe_mem, true_and]
+    rfl⟩
+
+lemma joinLiftRight_injective {φs : List 𝓕.States} {φsΛ : WickContraction φs.length}
+    {φsucΛ : WickContraction [φsΛ]ᵘᶜ.length} :
+    Function.Injective (@joinLiftRight _ _ φsΛ φsucΛ) := by
+  intro a b h
+  simp only [joinLiftRight] at h
+  rw [Subtype.mk_eq_mk] at h
+  simp only [Finset.map_inj] at h
+  refine Subtype.eq h
+
+lemma jointLiftLeft_disjoint_joinLiftRight {φs : List 𝓕.States} {φsΛ : WickContraction φs.length}
+    {φsucΛ : WickContraction [φsΛ]ᵘᶜ.length} (a : φsΛ.1) (b : φsucΛ.1) :
+    Disjoint (@joinLiftLeft _ _ _ φsucΛ a).1 (joinLiftRight b).1 := by
+  simp only [joinLiftLeft, joinLiftRight]
+  symm
+  apply uncontractedListEmd_finset_disjoint_left
+  exact a.2
+
+lemma jointLiftLeft_neq_joinLiftRight {φs : List 𝓕.States} {φsΛ : WickContraction φs.length}
+    {φsucΛ : WickContraction [φsΛ]ᵘᶜ.length} (a : φsΛ.1) (b : φsucΛ.1) :
+    joinLiftLeft a ≠ joinLiftRight b := by
+  by_contra hn
+  have h1 := jointLiftLeft_disjoint_joinLiftRight a b
+  rw [hn] at h1
+  simp at h1
+  have hj := (join φsΛ φsucΛ).2.1 (joinLiftRight b).1 (joinLiftRight b).2
+  rw [h1] at hj
+  simp at hj
+
+def joinLift {φs : List 𝓕.States} {φsΛ : WickContraction φs.length}
+    {φsucΛ : WickContraction [φsΛ]ᵘᶜ.length} : φsΛ.1 ⊕ φsucΛ.1 → (join φsΛ φsucΛ).1 := fun a =>
+  match a with
+  | Sum.inl a => joinLiftLeft a
+  | Sum.inr a => joinLiftRight a
+
+lemma joinLift_injective {φs : List 𝓕.States} {φsΛ : WickContraction φs.length}
+    {φsucΛ : WickContraction [φsΛ]ᵘᶜ.length} : Function.Injective (@joinLift _ _ φsΛ φsucΛ) := by
+  intro a b h
+  match a, b with
+  | Sum.inl a, Sum.inl b =>
+    simp
+    exact jointLiftLeft_injective h
+  | Sum.inr a, Sum.inr b =>
+    simp
+    exact joinLiftRight_injective h
+  | Sum.inl a, Sum.inr b =>
+    simp [joinLift] at h
+    have h1 := jointLiftLeft_neq_joinLiftRight a b
+    simp_all
+  | Sum.inr a, Sum.inl b =>
+    simp [joinLift] at h
+    have h1 := jointLiftLeft_neq_joinLiftRight b a
+    simp_all
+
+lemma joinLift_surjective {φs : List 𝓕.States} {φsΛ : WickContraction φs.length}
+    {φsucΛ : WickContraction [φsΛ]ᵘᶜ.length} : Function.Surjective (@joinLift _ _ φsΛ φsucΛ) := by
+  intro a
+  have ha2 := a.2
+  simp  [- Finset.coe_mem, join] at ha2
+  rcases ha2 with ha2 | ⟨a2, ha3⟩
+  · use Sum.inl ⟨a, ha2⟩
+    simp [joinLift, joinLiftLeft]
+  · rw [Finset.mapEmbedding_apply] at ha3
+    use Sum.inr ⟨a2, ha3.1⟩
+    simp [joinLift, joinLiftRight]
+    refine Subtype.eq ?_
+    exact ha3.2
+
+lemma joinLift_bijective {φs : List 𝓕.States} {φsΛ : WickContraction φs.length}
+    {φsucΛ : WickContraction [φsΛ]ᵘᶜ.length} : Function.Bijective (@joinLift _ _ φsΛ φsucΛ) := by
+  apply And.intro
+  · exact joinLift_injective
+  · exact joinLift_surjective
+
+lemma prod_join {φs : List 𝓕.States} (φsΛ : WickContraction φs.length)
+    (φsucΛ : WickContraction [φsΛ]ᵘᶜ.length) (f : (join φsΛ φsucΛ).1  → M) [ CommMonoid M]:
+      ∏ (a : (join φsΛ φsucΛ).1), f a = (∏ (a : φsΛ.1), f (joinLiftLeft a)) *
+      ∏ (a : φsucΛ.1), f (joinLiftRight a) := by
+  let e1 := Equiv.ofBijective (@joinLift _ _ φsΛ φsucΛ) joinLift_bijective
+  rw [← e1.prod_comp]
+  simp only [Fintype.prod_sum_type, Finset.univ_eq_attach]
+  rfl
+
+@[simp]
+lemma join_fstFieldOfContract_joinLiftRight {φs : List 𝓕.States} (φsΛ : WickContraction φs.length)
+    (φsucΛ : WickContraction [φsΛ]ᵘᶜ.length) (a : φsucΛ.1) :
+    (join φsΛ φsucΛ).fstFieldOfContract (joinLiftRight a) =
+    uncontractedListEmd (φsucΛ.fstFieldOfContract a) := by
+  apply eq_fstFieldOfContract_of_mem _ _ _ (uncontractedListEmd (φsucΛ.sndFieldOfContract a))
+  · simp [joinLiftRight]
+  · simp [joinLiftRight]
+  · apply uncontractedListEmd_strictMono
+    exact fstFieldOfContract_lt_sndFieldOfContract φsucΛ a
+
+@[simp]
+lemma join_sndFieldOfContract_joinLiftRight {φs : List 𝓕.States} (φsΛ : WickContraction φs.length)
+    (φsucΛ : WickContraction [φsΛ]ᵘᶜ.length) (a : φsucΛ.1) :
+    (join φsΛ φsucΛ).sndFieldOfContract (joinLiftRight a) =
+    uncontractedListEmd (φsucΛ.sndFieldOfContract a) := by
+  apply eq_sndFieldOfContract_of_mem _ _ (uncontractedListEmd (φsucΛ.fstFieldOfContract a))
+  · simp [joinLiftRight]
+  · simp [joinLiftRight]
+  · apply uncontractedListEmd_strictMono
+    exact fstFieldOfContract_lt_sndFieldOfContract φsucΛ a
+
+@[simp]
+lemma join_fstFieldOfContract_joinLiftLeft {φs : List 𝓕.States} (φsΛ : WickContraction φs.length)
+    (φsucΛ : WickContraction [φsΛ]ᵘᶜ.length) (a : φsΛ.1) :
+    (join φsΛ φsucΛ).fstFieldOfContract (joinLiftLeft a) =
+    (φsΛ.fstFieldOfContract a) := by
+  apply eq_fstFieldOfContract_of_mem _ _ _ (φsΛ.sndFieldOfContract a)
+  · simp [joinLiftLeft]
+  · simp [joinLiftLeft]
+  · exact fstFieldOfContract_lt_sndFieldOfContract φsΛ a
+
+@[simp]
+lemma join_sndFieldOfContract_joinLift {φs : List 𝓕.States} (φsΛ : WickContraction φs.length)
+    (φsucΛ : WickContraction [φsΛ]ᵘᶜ.length) (a : φsΛ.1) :
+    (join φsΛ φsucΛ).sndFieldOfContract (joinLiftLeft a) =
+    (φsΛ.sndFieldOfContract a) := by
+  apply eq_sndFieldOfContract_of_mem _ _ (φsΛ.fstFieldOfContract a) (φsΛ.sndFieldOfContract a)
+  · simp [joinLiftLeft]
+  · simp [joinLiftLeft]
+  · exact fstFieldOfContract_lt_sndFieldOfContract φsΛ a
+
+
+lemma join_card {φs : List 𝓕.States} {φsΛ : WickContraction φs.length}
+    {φsucΛ : WickContraction [φsΛ]ᵘᶜ.length} :
+    (join φsΛ φsucΛ).1.card = φsΛ.1.card + φsucΛ.1.card := by
+  simp [join]
+  rw [Finset.card_union_of_disjoint]
+  simp
+  rw [@Finset.disjoint_left]
+  intro a ha
+  simp
+  intro x hx
+  by_contra hn
+  have hdis : Disjoint (Finset.map uncontractedListEmd x)  a := by
+    exact uncontractedListEmd_finset_disjoint_left x a ha
+  rw [Finset.mapEmbedding_apply] at hn
+  rw [hn] at hdis
+  simp at hdis
+  have hcard := φsΛ.2.1 a ha
+  simp_all
+
+@[simp]
+lemma empty_join {φs : List 𝓕.States} (φsΛ : WickContraction [empty (n := φs.length)]ᵘᶜ.length) :
+    join empty φsΛ = congr (by simp) φsΛ := by
+  apply Subtype.ext
+  simp [join]
+  ext a
+  conv_lhs =>
+    left
+    left
+    rw [empty]
+  simp
+  rw [mem_congr_iff]
+  apply Iff.intro
+  · intro h
+    obtain ⟨a, ha, rfl⟩ := h
+    rw [Finset.mapEmbedding_apply]
+    rw [Finset.map_map]
+    apply Set.mem_of_eq_of_mem _ ha
+    trans Finset.map (Equiv.refl _).toEmbedding a
+    rfl
+    simp
+  · intro h
+    use Finset.map (finCongr (by simp)).toEmbedding a
+    simp [h]
+    trans Finset.map (Equiv.refl _).toEmbedding a
+    rw [Finset.mapEmbedding_apply, Finset.map_map]
+    rfl
+    simp
+
+@[simp]
+lemma join_empty {φs : List 𝓕.States} (φsΛ : WickContraction φs.length) :
+    join φsΛ empty = φsΛ := by
+  apply Subtype.ext
+  ext a
+  simp [join, empty]
+
+lemma join_timeContract {φs : List 𝓕.States} (φsΛ : WickContraction φs.length)
+    (φsucΛ : WickContraction [φsΛ]ᵘᶜ.length) :
+    (join φsΛ φsucΛ).timeContract = φsΛ.timeContract * φsucΛ.timeContract := by
+  simp only [timeContract, List.get_eq_getElem]
+  rw [prod_join]
+  congr 1
+  congr
+  funext a
+  simp
+
+lemma mem_join_uncontracted_of_mem_right_uncontracted {φs : List 𝓕.States}
+    (φsΛ : WickContraction φs.length)
+    (φsucΛ : WickContraction [φsΛ]ᵘᶜ.length) (i : Fin [φsΛ]ᵘᶜ.length)
+    (ha : i ∈ φsucΛ.uncontracted) :
+    uncontractedListEmd i ∈ (join φsΛ φsucΛ).uncontracted := by
+  rw [mem_uncontracted_iff_not_contracted]
+  intro p hp
+  simp [join] at hp
+  rcases hp with hp | hp
+  · have hi :  uncontractedListEmd i  ∈ φsΛ.uncontracted := by
+      exact uncontractedListEmd_mem_uncontracted i
+    rw [mem_uncontracted_iff_not_contracted] at hi
+    exact hi p hp
+  · obtain ⟨p, hp, rfl⟩ := hp
+    rw [Finset.mapEmbedding_apply]
+    simp
+    rw [mem_uncontracted_iff_not_contracted] at ha
+    exact ha p hp
+
+lemma exists_mem_left_uncontracted_of_mem_join_uncontracted {φs : List 𝓕.States}
+    (φsΛ : WickContraction φs.length)
+    (φsucΛ : WickContraction [φsΛ]ᵘᶜ.length) (i : Fin φs.length)
+    (ha : i ∈ (join φsΛ φsucΛ).uncontracted) :
+    i ∈ φsΛ.uncontracted := by
+  rw [@mem_uncontracted_iff_not_contracted]
+  rw [@mem_uncontracted_iff_not_contracted] at ha
+  simp [join] at ha
+  intro p hp
+  have hp' := ha p
+  simp_all
+
+lemma exists_mem_right_uncontracted_of_mem_join_uncontracted {φs : List 𝓕.States}
+    (φsΛ : WickContraction φs.length)
+    (φsucΛ : WickContraction [φsΛ]ᵘᶜ.length) (i : Fin φs.length)
+    (hi : i ∈ (join φsΛ φsucΛ).uncontracted) :
+    ∃ a, uncontractedListEmd a = i ∧ a ∈ φsucΛ.uncontracted := by
+  have hi' := exists_mem_left_uncontracted_of_mem_join_uncontracted _ _ i hi
+  obtain ⟨j, rfl⟩ := uncontractedListEmd_surjective_mem_uncontracted i hi'
+  use j
+  simp
+  rw [mem_uncontracted_iff_not_contracted] at hi
+  rw [mem_uncontracted_iff_not_contracted]
+  intro p hp
+  have hip := hi (p.map uncontractedListEmd) (by
+    simp [join]
+    right
+    use p
+    simp [hp]
+    rw [Finset.mapEmbedding_apply])
+  simpa using hip
+
+lemma join_uncontractedList {φs : List 𝓕.States} (φsΛ : WickContraction φs.length)
+    (φsucΛ : WickContraction [φsΛ]ᵘᶜ.length) :
+    (join φsΛ φsucΛ).uncontractedList = List.map uncontractedListEmd φsucΛ.uncontractedList := by
+  rw [uncontractedList_eq_sort]
+  rw [uncontractedList_eq_sort]
+  rw [fin_finset_sort_map_monotone]
+  congr
+  ext a
+  simp
+  apply Iff.intro
+  · intro h
+    obtain ⟨a, rfl, ha⟩ := exists_mem_right_uncontracted_of_mem_join_uncontracted _ _ a h
+    use a, ha
+  · intro h
+    obtain ⟨a, ha, rfl⟩ := h
+    exact mem_join_uncontracted_of_mem_right_uncontracted φsΛ φsucΛ a ha
+  · intro a b h
+    exact uncontractedListEmd_strictMono h
+
+lemma join_uncontractedList_get {φs : List 𝓕.States} (φsΛ : WickContraction φs.length)
+    (φsucΛ : WickContraction [φsΛ]ᵘᶜ.length) :
+    ((join φsΛ φsucΛ).uncontractedList).get =
+    φsΛ.uncontractedListEmd ∘  (φsucΛ.uncontractedList).get ∘ (
+        Fin.cast (by rw [join_uncontractedList]; simp) ):= by
+  have  h1 {n : ℕ} (l1 l2 : List (Fin  n)) (h : l1 = l2) :   l1.get = l2.get ∘ Fin.cast (by rw [h]):= by
+    subst h
+    rfl
+  have hl := h1 _ _ (join_uncontractedList φsΛ φsucΛ)
+  conv_lhs => rw [h1 _ _ (join_uncontractedList φsΛ φsucΛ)]
+  ext i
+  simp
+
+lemma join_uncontractedListGet {φs : List 𝓕.States} (φsΛ : WickContraction φs.length)
+    (φsucΛ : WickContraction [φsΛ]ᵘᶜ.length) :
+    (join φsΛ φsucΛ).uncontractedListGet = φsucΛ.uncontractedListGet := by
+  simp [uncontractedListGet, join_uncontractedList]
+  intro a ha
+  simp [uncontractedListEmd, uncontractedIndexEquiv]
+  rfl
+
+lemma join_uncontractedListEmb  {φs : List 𝓕.States} (φsΛ : WickContraction φs.length)
+    (φsucΛ : WickContraction [φsΛ]ᵘᶜ.length) :
+    (join φsΛ φsucΛ).uncontractedListEmd =
+    ((finCongr (congrArg List.length (join_uncontractedListGet _ _))).toEmbedding.trans φsucΛ.uncontractedListEmd).trans φsΛ.uncontractedListEmd := by
+  refine Function.Embedding.ext_iff.mpr (congrFun ?_)
+  change uncontractedListEmd.toFun = _
+  rw [uncontractedListEmd_toFun_eq_get]
+  rw [join_uncontractedList_get]
+  rfl
+
+lemma join_assoc {φs : List 𝓕.States} (φsΛ : WickContraction φs.length)
+    (φsucΛ : WickContraction [φsΛ]ᵘᶜ.length) (φsucΛ' : WickContraction [φsΛ.join φsucΛ]ᵘᶜ.length) :
+    join (join φsΛ φsucΛ) (φsucΛ') = join φsΛ (join φsucΛ (congr
+      (congrArg List.length (join_uncontractedListGet _ _)) φsucΛ')) := by
+  apply Subtype.ext
+  ext a
+  by_cases ha : a ∈ φsΛ.1
+  · simp [ha, join]
+  simp [ha, join]
+  apply Iff.intro
+  · intro h
+    rcases h with h | h
+    · obtain ⟨a, ha', rfl⟩ := h
+      use a
+      simp [ha']
+    · obtain ⟨a, ha', rfl⟩ := h
+      let a' := congrLift (congrArg List.length (join_uncontractedListGet _ _))  ⟨a, ha'⟩
+      let a'' := joinLiftRight  a'
+      use a''
+      apply And.intro
+      · right
+        use a'
+        apply And.intro
+        · exact a'.2
+        · simp only [joinLiftRight, a'']
+          rfl
+      · simp only [a'']
+        rw [Finset.mapEmbedding_apply, Finset.mapEmbedding_apply]
+        simp only [a', joinLiftRight, congrLift]
+        rw [join_uncontractedListEmb]
+        simp [Finset.map_map]
+  · intro h
+    obtain ⟨a, ha', rfl⟩ := h
+    rcases ha' with ha' | ha'
+    · left
+      use a
+    · obtain ⟨a, ha', rfl⟩ := ha'
+      right
+      let a' := congrLiftInv _ ⟨a, ha'⟩
+      use a'
+      simp
+      simp only [a']
+      rw [Finset.mapEmbedding_apply]
+      rw [join_uncontractedListEmb]
+      simp only [congrLiftInv, ← Finset.map_map]
+      congr
+      rw [Finset.map_map]
+      change Finset.map (Equiv.refl _).toEmbedding a = _
+      simp only [Equiv.refl_toEmbedding, Finset.map_refl]
+
+@[simp]
+lemma join_getDual?_apply_uncontractedListEmb_eq_none_iff  {φs : List 𝓕.States} (φsΛ : WickContraction φs.length)
+    (φsucΛ : WickContraction [φsΛ]ᵘᶜ.length) (i : Fin [φsΛ]ᵘᶜ.length) :
+    (join φsΛ φsucΛ).getDual?  (uncontractedListEmd i) = none
+    ↔ φsucΛ.getDual? i = none := by
+  rw [getDual?_eq_none_iff_mem_uncontracted, getDual?_eq_none_iff_mem_uncontracted]
+  apply Iff.intro
+  · intro h
+    obtain ⟨a, ha', ha⟩ := exists_mem_right_uncontracted_of_mem_join_uncontracted _ _ (uncontractedListEmd i) h
+    simp at ha'
+    subst ha'
+    exact ha
+  · intro h
+    exact mem_join_uncontracted_of_mem_right_uncontracted φsΛ φsucΛ i h
+
+@[simp]
+lemma join_getDual?_apply_uncontractedListEmb_isSome_iff {φs : List 𝓕.States} (φsΛ : WickContraction φs.length)
+    (φsucΛ : WickContraction [φsΛ]ᵘᶜ.length) (i : Fin [φsΛ]ᵘᶜ.length) :
+     ((join φsΛ φsucΛ).getDual?  (uncontractedListEmd i)).isSome
+    ↔ (φsucΛ.getDual? i).isSome := by
+  rw [← Decidable.not_iff_not]
+  simp
+
+lemma join_getDual?_apply_uncontractedListEmb_some {φs : List 𝓕.States} (φsΛ : WickContraction φs.length)
+    (φsucΛ : WickContraction [φsΛ]ᵘᶜ.length) (i : Fin [φsΛ]ᵘᶜ.length)
+    (hi :((join φsΛ φsucΛ).getDual?  (uncontractedListEmd i)).isSome) :
+    ((join φsΛ φsucΛ).getDual?  (uncontractedListEmd i)) =
+    some (uncontractedListEmd ((φsucΛ.getDual? i).get (by simpa using hi)))  := by
+  rw [getDual?_eq_some_iff_mem]
+  simp [join]
+  right
+  use {i, (φsucΛ.getDual? i).get (by simpa using hi)}
+  simp
+  rw [Finset.mapEmbedding_apply]
+  simp
+
+@[simp]
+lemma join_getDual?_apply_uncontractedListEmb {φs : List 𝓕.States} (φsΛ : WickContraction φs.length)
+    (φsucΛ : WickContraction [φsΛ]ᵘᶜ.length) (i : Fin [φsΛ]ᵘᶜ.length) :
+    ((join φsΛ φsucΛ).getDual?  (uncontractedListEmd i)) = Option.map uncontractedListEmd (φsucΛ.getDual? i) := by
+  by_cases h : (φsucΛ.getDual? i).isSome
+  · rw [join_getDual?_apply_uncontractedListEmb_some]
+    have h1 : (φsucΛ.getDual? i)  =(φsucΛ.getDual? i).get (by simpa using h) :=
+      Eq.symm (Option.some_get h)
+    conv_rhs => rw [h1]
+    simp  [- Option.some_get]
+    exact (join_getDual?_apply_uncontractedListEmb_isSome_iff φsΛ φsucΛ i).mpr h
+  · simp only [Bool.not_eq_true, Option.not_isSome, Option.isNone_iff_eq_none] at h
+    rw [h]
+    simp
+    exact h
+
+/-!
+
+## Subcontractions and quotient contractions
+
+-/
+
+section
+
+variable {φs : List 𝓕.States} (φsΛ : WickContraction φs.length)
+
+lemma join_sub_quot (S : Finset (Finset (Fin φs.length))) (ha : S ⊆ φsΛ.1) :
+    join (subContraction S ha) (quotContraction S ha) = φsΛ := by
+  apply Subtype.ext
+  ext a
+  simp [join]
+  apply Iff.intro
+  · intro h
+    rcases h with h | h
+    · exact mem_of_mem_subContraction h
+    · obtain ⟨a, ha, rfl⟩ := h
+      apply mem_of_mem_quotContraction ha
+  · intro h
+    have h1 := mem_subContraction_or_quotContraction (S := S) (a := a) (hs := ha) h
+    rcases h1 with h1 | h1
+    · simp [h1]
+    · right
+      obtain ⟨a, rfl, ha⟩ := h1
+      use a
+      simp [ha]
+      rw [Finset.mapEmbedding_apply]
+
+lemma subContraction_card_plus_quotContraction_card_eq (S : Finset (Finset (Fin φs.length)))
+    (ha : S ⊆ φsΛ.1) :
+    (subContraction S ha).1.card + (quotContraction S ha).1.card = φsΛ.1.card := by
+  rw [← join_card]
+  simp [join_sub_quot]
+
+end
+open FieldStatistic
+
+lemma stat_signFinset_right {φs : List 𝓕.States} (φsΛ : WickContraction φs.length)
+    (φsucΛ : WickContraction [φsΛ]ᵘᶜ.length) (i j : Fin [φsΛ]ᵘᶜ.length) :
+    (𝓕 |>ₛ ⟨[φsΛ]ᵘᶜ.get, φsucΛ.signFinset i j⟩) =
+    (𝓕 |>ₛ ⟨φs.get, (φsucΛ.signFinset i j).map uncontractedListEmd⟩) := by
+  simp [ofFinset]
+  congr 1
+  rw [← fin_finset_sort_map_monotone]
+  simp
+  intro i j h
+  exact uncontractedListEmd_strictMono h
+
+lemma signFinset_right_map_uncontractedListEmd_eq_filter {φs : List 𝓕.States}
+    (φsΛ : WickContraction φs.length) (φsucΛ : WickContraction [φsΛ]ᵘᶜ.length)
+    (i j : Fin [φsΛ]ᵘᶜ.length) : (φsucΛ.signFinset i j).map uncontractedListEmd =
+    ((join φsΛ φsucΛ).signFinset (uncontractedListEmd i) (uncontractedListEmd j)).filter
+    (fun c => c ∈ φsΛ.uncontracted) := by
+  ext a
+  simp
+  apply Iff.intro
+  · intro h
+    obtain ⟨a, ha, rfl⟩ := h
+    apply And.intro
+    · simp_all [signFinset]
+      apply And.intro
+      · exact uncontractedListEmd_strictMono ha.1
+      · apply And.intro
+        · exact uncontractedListEmd_strictMono ha.2.1
+        · have ha2 := ha.2.2
+          simp_all
+          rcases ha2 with ha2 | ha2
+          · simp [ha2]
+          · right
+            intro h
+            have h1 : (φsucΛ.getDual? a) = some ((φsucΛ.getDual? a).get h) :=
+              Eq.symm (Option.some_get h)
+            apply lt_of_lt_of_eq (uncontractedListEmd_strictMono (ha2 h))
+            rw [Option.get_map]
+    · exact uncontractedListEmd_mem_uncontracted a
+  · intro h
+    have h2 := h.2
+    have h2' := uncontractedListEmd_surjective_mem_uncontracted a h.2
+    obtain ⟨a, rfl⟩ := h2'
+    use a
+    have h1 := h.1
+    simp_all [signFinset]
+    apply And.intro
+    · have h1 := h.1
+      rw [StrictMono.lt_iff_lt] at h1
+      exact h1
+      exact fun _ _ h => uncontractedListEmd_strictMono h
+    · apply And.intro
+      · have h1 := h.2.1
+        rw [StrictMono.lt_iff_lt] at h1
+        exact h1
+        exact fun _ _ h => uncontractedListEmd_strictMono h
+      · have h1 := h.2.2
+        simp_all
+        rcases h1 with h1 | h1
+        · simp [h1]
+        · right
+          intro h
+          have h1' := h1 h
+          have hl : uncontractedListEmd i < uncontractedListEmd ((φsucΛ.getDual? a).get h) := by
+            apply lt_of_lt_of_eq h1'
+            simp [Option.get_map]
+          rw [StrictMono.lt_iff_lt] at hl
+          exact hl
+          exact fun _ _ h => uncontractedListEmd_strictMono h
+
+lemma sign_right_eq_prod_mul_prod {φs : List 𝓕.States} (φsΛ : WickContraction φs.length)
+    (φsucΛ : WickContraction [φsΛ]ᵘᶜ.length) :
+    φsucΛ.sign = (∏ a, 𝓢(𝓕|>ₛ [φsΛ]ᵘᶜ[φsucΛ.sndFieldOfContract a], 𝓕|>ₛ ⟨φs.get ,
+    ((join φsΛ φsucΛ).signFinset (uncontractedListEmd (φsucΛ.fstFieldOfContract a)) (uncontractedListEmd (φsucΛ.sndFieldOfContract a))).filter
+      (fun c => ¬  c ∈ φsΛ.uncontracted)⟩)) *
+    (∏ a, 𝓢(𝓕|>ₛ [φsΛ]ᵘᶜ[φsucΛ.sndFieldOfContract a], 𝓕|>ₛ ⟨φs.get ,
+      ((join φsΛ φsucΛ).signFinset (uncontractedListEmd (φsucΛ.fstFieldOfContract a))
+        (uncontractedListEmd (φsucΛ.sndFieldOfContract a)))⟩)) := by
+  rw [← Finset.prod_mul_distrib, sign]
+  congr
+  funext a
+  rw [← map_mul]
+  congr
+  rw [stat_signFinset_right, signFinset_right_map_uncontractedListEmd_eq_filter]
+  rw [ofFinset_filter]
+
+lemma join_singleton_signFinset_eq_filter {φs : List 𝓕.States}
+    {i j : Fin φs.length} (h : i < j)
+    (φsucΛ : WickContraction [singleton h]ᵘᶜ.length)  :
+    (join (singleton h) φsucΛ).signFinset i j =
+    ((singleton h).signFinset i j).filter (fun c => ¬
+    (((join (singleton h) φsucΛ).getDual? c).isSome ∧
+    ((h1 : ((join (singleton h) φsucΛ).getDual? c).isSome) →
+    (((join (singleton h) φsucΛ).getDual? c).get h1) < i))) := by
+  ext a
+  simp [signFinset, and_assoc]
+  intro h1 h2
+  have h1 : (singleton h).getDual? a = none  := by
+    rw [singleton_getDual?_eq_none_iff_neq]
+    omega
+  simp [h1]
+  apply Iff.intro
+  · intro h1 h2
+    rcases h1 with h1 | h1
+    · simp [h1]
+      have h2' : ¬  (((singleton h).join φsucΛ).getDual? a).isSome := by
+        exact Option.not_isSome_iff_eq_none.mpr h1
+      exact h2' h2
+    use h2
+    have h1 := h1 h2
+    omega
+  · intro h2
+    by_cases h2' :  (((singleton h).join φsucΛ).getDual? a).isSome = true
+    · have h2 := h2 h2'
+      obtain ⟨hb, h2⟩ := h2
+      right
+      intro hl
+      apply lt_of_le_of_ne h2
+      by_contra hn
+      have hij : ((singleton h).join φsucΛ).getDual? i = j := by
+        rw [@getDual?_eq_some_iff_mem]
+        simp [join, singleton]
+      simp [hn] at hij
+      omega
+    · simp at h2'
+      simp [h2']
+
+
+lemma join_singleton_left_signFinset_eq_filter {φs : List 𝓕.States}
+    {i j : Fin φs.length} (h : i < j)
+    (φsucΛ : WickContraction [singleton h]ᵘᶜ.length)  :
+    (𝓕 |>ₛ ⟨φs.get, (singleton h).signFinset i j⟩)
+    = (𝓕 |>ₛ ⟨φs.get, (join (singleton h) φsucΛ).signFinset i j⟩) *
+      (𝓕 |>ₛ ⟨φs.get, ((singleton h).signFinset i j).filter (fun c =>
+      (((join (singleton h) φsucΛ).getDual? c).isSome ∧
+      ((h1 : ((join (singleton h) φsucΛ).getDual? c).isSome) →
+      (((join (singleton h) φsucΛ).getDual? c).get h1) < i)))⟩) := by
+  conv_rhs =>
+    left
+    rw [join_singleton_signFinset_eq_filter]
+  rw [mul_comm]
+  exact (ofFinset_filter_mul_neg 𝓕.statesStatistic _ _ _).symm
+
+def joinSignRightExtra {φs : List 𝓕.States}
+    {i j : Fin φs.length} (h : i < j)
+    (φsucΛ : WickContraction [singleton h]ᵘᶜ.length)  : ℂ :=
+    ∏ a, 𝓢(𝓕|>ₛ [singleton h]ᵘᶜ[φsucΛ.sndFieldOfContract a], 𝓕|>ₛ ⟨φs.get ,
+    ((join (singleton h) φsucΛ).signFinset (uncontractedListEmd (φsucΛ.fstFieldOfContract a))
+    (uncontractedListEmd (φsucΛ.sndFieldOfContract a))).filter
+    (fun c => ¬  c ∈ (singleton h).uncontracted)⟩)
+
+
+def joinSignLeftExtra {φs : List 𝓕.States}
+    {i j : Fin φs.length} (h : i < j)
+    (φsucΛ : WickContraction [singleton h]ᵘᶜ.length)  : ℂ :=
+    𝓢(𝓕 |>ₛ φs[j], (𝓕 |>ₛ ⟨φs.get, ((singleton h).signFinset i j).filter (fun c =>
+      (((join (singleton h) φsucΛ).getDual? c).isSome ∧
+      ((h1 : ((join (singleton h) φsucΛ).getDual? c).isSome) →
+      (((join (singleton h) φsucΛ).getDual? c).get h1) < i)))⟩))
+
+lemma join_singleton_sign_left {φs : List 𝓕.States}
+    {i j : Fin φs.length} (h : i < j)
+    (φsucΛ : WickContraction [singleton h]ᵘᶜ.length)  :
+    (singleton h).sign = 𝓢(𝓕 |>ₛ φs[j], (𝓕 |>ₛ ⟨φs.get, (join (singleton h) φsucΛ).signFinset i j⟩)) *
+    (joinSignLeftExtra h φsucΛ) := by
+  rw [singleton_sign_expand]
+  rw [join_singleton_left_signFinset_eq_filter h φsucΛ]
+  rw [map_mul]
+  rfl
+
+
+lemma join_singleton_sign_right {φs : List 𝓕.States}
+    {i j : Fin φs.length} (h : i < j)
+    (φsucΛ : WickContraction [singleton h]ᵘᶜ.length)  :
+    φsucΛ.sign =
+    (joinSignRightExtra h φsucΛ) *
+    (∏ a, 𝓢(𝓕|>ₛ [singleton h]ᵘᶜ[φsucΛ.sndFieldOfContract a], 𝓕|>ₛ ⟨φs.get ,
+      ((join (singleton h) φsucΛ).signFinset (uncontractedListEmd (φsucΛ.fstFieldOfContract a))
+        (uncontractedListEmd (φsucΛ.sndFieldOfContract a)))⟩))  := by
+  rw [sign_right_eq_prod_mul_prod]
+  rfl
+
+@[simp]
+lemma join_singleton_getDual?_left {φs : List 𝓕.States}
+    {i j : Fin φs.length} (h : i < j)
+    (φsucΛ : WickContraction [singleton h]ᵘᶜ.length)  :
+    (join (singleton h) φsucΛ).getDual? i = some j := by
+  rw [@getDual?_eq_some_iff_mem]
+  simp [singleton, join]
+
+@[simp]
+lemma join_singleton_getDual?_right {φs : List 𝓕.States}
+    {i j : Fin φs.length} (h : i < j)
+    (φsucΛ : WickContraction [singleton h]ᵘᶜ.length)  :
+    (join (singleton h) φsucΛ).getDual? j = some i := by
+  rw [@getDual?_eq_some_iff_mem]
+  simp [singleton, join]
+  left
+  exact Finset.pair_comm j i
+
+
+lemma joinSignRightExtra_eq_i_j_finset_eq_if {φs : List 𝓕.States}
+    {i j : Fin φs.length} (h : i < j)
+    (φsucΛ : WickContraction [singleton h]ᵘᶜ.length)  :
+    joinSignRightExtra h φsucΛ = ∏ a,
+    𝓢((𝓕|>ₛ [singleton h]ᵘᶜ[φsucΛ.sndFieldOfContract a]),
+    𝓕 |>ₛ ⟨φs.get, (if uncontractedListEmd (φsucΛ.fstFieldOfContract a) < j ∧
+        j < uncontractedListEmd (φsucΛ.sndFieldOfContract a) ∧
+        uncontractedListEmd (φsucΛ.fstFieldOfContract a) < i  then {j} else ∅)
+        ∪ (if uncontractedListEmd (φsucΛ.fstFieldOfContract a) < i ∧
+        i < uncontractedListEmd (φsucΛ.sndFieldOfContract a)  then {i} else ∅)⟩) := by
+  rw [joinSignRightExtra]
+  congr
+  funext a
+  congr
+  rw [signFinset]
+  rw [Finset.filter_comm]
+  have h11 : (Finset.filter (fun c => c ∉ (singleton h).uncontracted) Finset.univ) = {i, j} := by
+    ext x
+    simp
+    rw [@mem_uncontracted_iff_not_contracted]
+    simp [singleton]
+    omega
+  rw [h11]
+  ext x
+  simp
+  have hjneqfst := singleton_uncontractedEmd_neq_right h (φsucΛ.fstFieldOfContract a)
+  have hjneqsnd := singleton_uncontractedEmd_neq_right h (φsucΛ.sndFieldOfContract a)
+  have hineqfst := singleton_uncontractedEmd_neq_left h (φsucΛ.fstFieldOfContract a)
+  have hineqsnd := singleton_uncontractedEmd_neq_left h (φsucΛ.sndFieldOfContract a)
+  by_cases hj1 : ¬ uncontractedListEmd (φsucΛ.fstFieldOfContract a) < j
+  · simp [hj1]
+    have hi1 : ¬ uncontractedListEmd (φsucΛ.fstFieldOfContract a) < i := by omega
+    simp [hi1]
+    intro hxij h1 h2
+    omega
+  · have hj1 : uncontractedListEmd (φsucΛ.fstFieldOfContract a) < j := by
+      omega
+    by_cases hi1 : ¬ i < uncontractedListEmd (φsucΛ.sndFieldOfContract a)
+    · simp [hi1]
+      have hj2 : ¬ j < uncontractedListEmd (φsucΛ.sndFieldOfContract a) := by omega
+      simp [hj2]
+      intro hxij h1 h2
+      omega
+    · have hi1 : i < uncontractedListEmd (φsucΛ.sndFieldOfContract a) := by
+        omega
+      simp [hi1, hj1]
+      by_cases hi2 : ¬  uncontractedListEmd (φsucΛ.fstFieldOfContract a) < i
+      · simp [hi2]
+        by_cases hj3 : ¬ j < uncontractedListEmd (φsucΛ.sndFieldOfContract a)
+        · omega
+        · have hj4 : j < uncontractedListEmd (φsucΛ.sndFieldOfContract a) := by omega
+          intro h
+          rcases h with h | h
+          · subst h
+            omega
+          · subst h
+            simp
+            omega
+      · have hi2 : uncontractedListEmd (φsucΛ.fstFieldOfContract a) < i := by omega
+        simp [hi2]
+        by_cases hj3 : ¬ j < uncontractedListEmd (φsucΛ.sndFieldOfContract a)
+        · simp [hj3]
+          apply Iff.intro
+          · intro h
+            omega
+          · intro h
+            subst h
+            simp
+            omega
+        · have hj3 : j < uncontractedListEmd (φsucΛ.sndFieldOfContract a) := by omega
+          simp [hj3]
+          apply Iff.intro
+          · intro h
+            omega
+          · intro h
+            rcases h with h1 | h1
+            · subst h1
+              simp
+              omega
+            · subst h1
+              simp
+              omega
+
+
+lemma joinSignLeftExtra_eq_joinSignRightExtra {φs : List 𝓕.States}
+    {i j : Fin φs.length} (h : i < j) (hs : (𝓕 |>ₛ φs[i]) = (𝓕 |>ₛ φs[j]))
+    (φsucΛ : WickContraction [singleton h]ᵘᶜ.length) :
+    joinSignLeftExtra h φsucΛ = joinSignRightExtra h φsucΛ := by
+  /- Simplifying joinSignLeftExtra. -/
+  rw [joinSignLeftExtra]
+  rw [ofFinset_eq_prod]
+  rw [map_prod]
+  let e2 : Fin φs.length ≃ {x // (((singleton h).join φsucΛ).getDual? x).isSome} ⊕ {x // ¬ (((singleton h).join φsucΛ).getDual? x).isSome} := by
+    exact (Equiv.sumCompl fun a => (((singleton h).join φsucΛ).getDual? a).isSome = true).symm
+  rw [← e2.symm.prod_comp]
+  simp only [Fin.getElem_fin, Fintype.prod_sum_type, instCommGroup]
+  conv_lhs =>
+    enter [2, 2, x]
+    simp only [Equiv.symm_symm, Equiv.sumCompl_apply_inl, Equiv.sumCompl_apply_inr, e2]
+    rw [if_neg (
+        by
+        simp
+        intro h1 h2
+        have hx := x.2
+        simp_all)]
+  simp
+  rw [← ((singleton h).join φsucΛ).sigmaContractedEquiv.prod_comp]
+  erw [Finset.prod_sigma]
+  conv_lhs =>
+    enter [2, a]
+    rw [prod_finset_eq_mul_fst_snd]
+    simp [e2, sigmaContractedEquiv]
+  rw [prod_join]
+  rw [singleton_prod]
+  simp only [join_fstFieldOfContract_joinLiftLeft, singleton_fstFieldOfContract,
+    join_sndFieldOfContract_joinLift, singleton_sndFieldOfContract, lt_self_iff_false, and_false,
+    ↓reduceIte, map_one, mul_one, join_fstFieldOfContract_joinLiftRight,
+    join_sndFieldOfContract_joinLiftRight, getElem_uncontractedListEmd]
+  rw [if_neg (by omega)]
+  simp only [map_one, one_mul]
+  /- Introducing joinSignRightExtra. -/
+  rw [joinSignRightExtra_eq_i_j_finset_eq_if]
+  congr
+  funext a
+  have hjneqfst := singleton_uncontractedEmd_neq_right h (φsucΛ.fstFieldOfContract a)
+  have hjneqsnd := singleton_uncontractedEmd_neq_right h (φsucΛ.sndFieldOfContract a)
+  have hineqfst := singleton_uncontractedEmd_neq_left h (φsucΛ.fstFieldOfContract a)
+  have hineqsnd := singleton_uncontractedEmd_neq_left h (φsucΛ.sndFieldOfContract a)
+  have hl : uncontractedListEmd (φsucΛ.fstFieldOfContract a) < uncontractedListEmd (φsucΛ.sndFieldOfContract a)  := by
+    apply uncontractedListEmd_strictMono
+    exact fstFieldOfContract_lt_sndFieldOfContract φsucΛ a
+  by_cases hj1 : ¬ uncontractedListEmd (φsucΛ.fstFieldOfContract a) < j
+  · have hi1 : ¬ uncontractedListEmd (φsucΛ.fstFieldOfContract a) < i := by omega
+    simp [hj1, hi1]
+  · have hj1 : uncontractedListEmd (φsucΛ.fstFieldOfContract a) < j := by omega
+    simp [hj1]
+    by_cases hi2 : ¬ i < uncontractedListEmd (φsucΛ.sndFieldOfContract a)
+    · have hi1 :  ¬ i < uncontractedListEmd (φsucΛ.fstFieldOfContract a) := by omega
+      have hj2 : ¬ j < uncontractedListEmd (φsucΛ.sndFieldOfContract a) := by omega
+      simp [hi2, hj2, hi1]
+    · have hi2 : i < uncontractedListEmd (φsucΛ.sndFieldOfContract a) := by omega
+      have hi2n : ¬ uncontractedListEmd (φsucΛ.sndFieldOfContract a) < i := by omega
+      simp [hi2, hi2n]
+      by_cases hj2 : ¬ j < uncontractedListEmd (φsucΛ.sndFieldOfContract a)
+      · simp [hj2]
+        have hj2 :  uncontractedListEmd (φsucΛ.sndFieldOfContract a) < j:= by omega
+        simp [hj2]
+        by_cases hi1 : ¬ uncontractedListEmd (φsucΛ.fstFieldOfContract a) < i
+        · simp [hi1]
+        · have hi1 : uncontractedListEmd (φsucΛ.fstFieldOfContract a) < i := by omega
+          simp [hi1, ofFinset_singleton]
+          erw [hs]
+          exact exchangeSign_symm (𝓕|>ₛφs[↑j]) (𝓕|>ₛ[singleton h]ᵘᶜ[↑(φsucΛ.sndFieldOfContract a)])
+      · simp  at hj2
+        simp [hj2]
+        by_cases hi1 : ¬ uncontractedListEmd (φsucΛ.fstFieldOfContract a) < i
+        · simp [hi1]
+        · have hi1 : uncontractedListEmd (φsucΛ.fstFieldOfContract a) < i := by omega
+          simp [hi1]
+          have hj2 : ¬  uncontractedListEmd (φsucΛ.sndFieldOfContract a) < j := by omega
+          simp [hj2]
+          rw [← ofFinset_union_disjoint]
+          simp only [instCommGroup, ofFinset_singleton, List.get_eq_getElem, hs]
+          erw [hs]
+          simp
+          simp
+          omega
+
+lemma join_sign_singleton {φs : List 𝓕.States}
+    {i j : Fin φs.length} (h : i < j) (hs : (𝓕 |>ₛ φs[i]) = (𝓕 |>ₛ φs[j]))
+    (φsucΛ : WickContraction [singleton h]ᵘᶜ.length) :
+    (join (singleton h) φsucΛ).sign = (singleton h).sign * φsucΛ.sign := by
+  rw [join_singleton_sign_right]
+  rw [join_singleton_sign_left h φsucΛ]
+  rw [joinSignLeftExtra_eq_joinSignRightExtra h hs φsucΛ]
+  rw [← mul_assoc]
+  rw [mul_assoc _ _ (joinSignRightExtra h φsucΛ)]
+  have h1 : (joinSignRightExtra h φsucΛ * joinSignRightExtra h φsucΛ) = 1 := by
+    rw [← joinSignLeftExtra_eq_joinSignRightExtra h hs φsucΛ]
+    simp [joinSignLeftExtra]
+  simp only [instCommGroup, Fin.getElem_fin, h1, mul_one]
+  rw [sign]
+  rw [prod_join]
+  congr
+  · rw [singleton_prod]
+    simp
+  · funext a
+    simp
+
+lemma exists_contraction_pair_of_card_ge_zero {φs : List 𝓕.States} (φsΛ : WickContraction φs.length)
+    (h : 0 < φsΛ.1.card) :
+    ∃ a, a ∈ φsΛ.1 := by
+  simpa using h
+
+lemma exists_join_singleton_of_card_ge_zero {φs : List 𝓕.States} (φsΛ : WickContraction φs.length)
+    (h : 0 < φsΛ.1.card) (hc : φsΛ.GradingCompliant) :
+    ∃ (i j : Fin φs.length) (h : i < j) (φsucΛ : WickContraction [singleton h]ᵘᶜ.length),
+    φsΛ = join (singleton h) φsucΛ ∧ (𝓕 |>ₛ φs[i]) = (𝓕 |>ₛ φs[j])
+    ∧ φsucΛ.GradingCompliant ∧ φsucΛ.1.card + 1 = φsΛ.1.card := by
+  obtain ⟨a, ha⟩ := exists_contraction_pair_of_card_ge_zero φsΛ h
+  use φsΛ.fstFieldOfContract ⟨a, ha⟩
+  use φsΛ.sndFieldOfContract ⟨a, ha⟩
+  use φsΛ.fstFieldOfContract_lt_sndFieldOfContract ⟨a, ha⟩
+  let φsucΛ :
+     WickContraction [singleton (φsΛ.fstFieldOfContract_lt_sndFieldOfContract ⟨a, ha⟩)]ᵘᶜ.length :=
+     congr (by simp [← subContraction_singleton_eq_singleton]) (φsΛ.quotContraction {a} (by simpa using ha))
+  use φsucΛ
+  simp [← subContraction_singleton_eq_singleton]
+  apply And.intro
+  · have h1 := join_congr (subContraction_singleton_eq_singleton _ ⟨a, ha⟩).symm (φsucΛ := φsucΛ)
+    simp [h1, φsucΛ]
+    rw [join_sub_quot]
+  · apply And.intro  (hc ⟨a, ha⟩)
+    apply And.intro
+    · simp [φsucΛ]
+      rw [gradingCompliant_congr (φs' := [(φsΛ.subContraction {a} (by simpa using ha))]ᵘᶜ)]
+      simp
+      exact quotContraction_gradingCompliant hc
+      rw [← subContraction_singleton_eq_singleton]
+    · simp [φsucΛ]
+      have h1 := subContraction_card_plus_quotContraction_card_eq _ {a} (by simpa using ha)
+      simp [subContraction] at h1
+      omega
+
+lemma join_sign_induction {φs : List 𝓕.States} (φsΛ : WickContraction φs.length)
+    (φsucΛ : WickContraction [φsΛ]ᵘᶜ.length) (hc : φsΛ.GradingCompliant) :
+    (n : ℕ) → (hn : φsΛ.1.card = n) →
+    (join φsΛ φsucΛ).sign = φsΛ.sign * φsucΛ.sign
+  | 0, hn => by
+    rw [@card_zero_iff_empty] at hn
+    subst hn
+    simp [sign_empty]
+    apply sign_congr
+    simp
+  | Nat.succ n, hn => by
+    obtain ⟨i, j, hij, φsucΛ', rfl, h1, h2, h3⟩ := exists_join_singleton_of_card_ge_zero φsΛ (by simp [hn]) hc
+    rw [join_assoc]
+    rw [join_sign_singleton hij h1 ]
+    rw [join_sign_singleton hij h1 ]
+    have hn : φsucΛ'.1.card = n   := by
+      omega
+    rw [join_sign_induction φsucΛ' (congr (by simp [join_uncontractedListGet]) φsucΛ) h2
+      n hn]
+    rw [mul_assoc]
+    simp [sign_congr]
+    left
+    left
+    apply sign_congr
+    exact join_uncontractedListGet (singleton hij) φsucΛ'
+
+lemma join_sign {φs : List 𝓕.States} (φsΛ : WickContraction φs.length)
+    (φsucΛ : WickContraction [φsΛ]ᵘᶜ.length) (hc : φsΛ.GradingCompliant) :
+    (join φsΛ φsucΛ).sign = φsΛ.sign * φsucΛ.sign := by
+  exact join_sign_induction φsΛ φsucΛ hc (φsΛ).1.card rfl
+
+end WickContraction
