HepLean/PerturbationTheory/WickContraction/Singleton.lean
@@ -1,0 +1,125 @@
+/-
+Copyright (c) 2025 Joseph Tooby-Smith. All rights reserved.
+Released under Apache 2.0 license as described in the file LICENSE.
+Authors: Joseph Tooby-Smith
+-/
+import HepLean.PerturbationTheory.WickContraction.TimeContract
+import HepLean.PerturbationTheory.WickContraction.StaticContract
+import HepLean.PerturbationTheory.Algebras.FieldOpAlgebra.TimeContraction
+import HepLean.PerturbationTheory.WickContraction.SubContraction
+/-!
+
+# Singleton of contractions
+
+-/
+
+open FieldSpecification
+variable {𝓕 : FieldSpecification}
+
+namespace WickContraction
+variable {n : ℕ} (c : WickContraction n)
+open HepLean.List
+open FieldOpAlgebra
+open FieldStatistic
+
+def singleton {i j : Fin n} (hij : i < j) : WickContraction n :=
+  ⟨{{i, j}}, by
+    intro i hi
+    simp at hi
+    subst hi
+    rw [@Finset.card_eq_two]
+    use i, j
+    simp
+    omega
+    , by
+    intro i hi j hj
+    simp_all⟩
+
+lemma mem_singleton {i j : Fin n} (hij : i < j) :
+    {i, j} ∈ (singleton  hij).1  := by
+  simp [singleton]
+
+lemma mem_singleton_iff {i j : Fin n} (hij : i < j) {a : Finset (Fin n)} :
+    a ∈ (singleton  hij).1 ↔ a = {i, j}  := by
+  simp [singleton]
+
+@[simp]
+lemma of_singleton_eq {i j : Fin n} (hij : i < j) (a : (singleton hij).1):
+    a = ⟨{i, j}, mem_singleton hij⟩ := by
+  have ha2 := a.2
+  rw [@mem_singleton_iff] at ha2
+  exact Subtype.coe_eq_of_eq_mk ha2
+
+lemma singleton_prod {φs : List 𝓕.States} {i j : Fin φs.length} (hij : i < j)
+    (f : (singleton hij).1 → M) [CommMonoid M]  :
+    ∏ a, f a = f ⟨{i,j}, mem_singleton hij⟩:= by
+  simp [singleton]
+
+@[simp]
+lemma singleton_fstFieldOfContract {i j : Fin n} (hij : i < j) :
+    (singleton hij).fstFieldOfContract ⟨{i, j}, mem_singleton hij⟩ = i := by
+  refine eq_fstFieldOfContract_of_mem (singleton hij) ⟨{i, j}, mem_singleton hij⟩ i j ?_ ?_ ?_
+  · simp
+  · simp
+  · exact hij
+
+@[simp]
+lemma singleton_sndFieldOfContract {i j : Fin n} (hij : i < j) :
+    (singleton hij).sndFieldOfContract ⟨{i, j}, mem_singleton hij⟩ = j := by
+  refine eq_sndFieldOfContract_of_mem (singleton hij) ⟨{i, j}, mem_singleton hij⟩ i j ?_ ?_ ?_
+  · simp
+  · simp
+  · exact hij
+
+lemma singleton_sign_expand {φs : List 𝓕.States} {i j : Fin φs.length} (hij : i < j) :
+    (singleton hij).sign = 𝓢(𝓕 |>ₛ φs[j], 𝓕 |>ₛ ⟨φs.get, (singleton hij).signFinset i j⟩) := by
+  rw [sign, singleton_prod]
+  simp
+
+lemma singleton_getDual?_eq_none_iff_neq {i j : Fin n} (hij : i < j) (a : Fin n) :
+    (singleton hij).getDual? a = none ↔ (i ≠ a ∧ j ≠ a) := by
+  rw [getDual?_eq_none_iff_mem_uncontracted]
+  rw [mem_uncontracted_iff_not_contracted]
+  simp [singleton]
+  omega
+
+lemma singleton_uncontractedEmd_neq_left {φs : List 𝓕.States} {i j : Fin φs.length} (hij : i < j)
+    (a : Fin [singleton hij]ᵘᶜ.length ) :
+    (singleton hij).uncontractedListEmd a ≠ i  := by
+  by_contra hn
+  have h1 : (singleton hij).uncontractedListEmd a ∈ (singleton hij).uncontracted := by
+    simp [uncontractedListEmd]
+  have h2 : i ∉  (singleton hij).uncontracted := by
+    rw [mem_uncontracted_iff_not_contracted]
+    simp [singleton]
+  simp_all
+
+lemma singleton_uncontractedEmd_neq_right {φs : List 𝓕.States} {i j : Fin φs.length} (hij : i < j)
+    (a : Fin [singleton hij]ᵘᶜ.length ) :
+    (singleton hij).uncontractedListEmd a ≠ j  := by
+  by_contra hn
+  have h1 : (singleton hij).uncontractedListEmd a ∈ (singleton hij).uncontracted := by
+    simp [uncontractedListEmd]
+  have h2 : j ∉  (singleton hij).uncontracted := by
+    rw [mem_uncontracted_iff_not_contracted]
+    simp [singleton]
+  simp_all
+
+@[simp]
+lemma mem_signFinset {i j : Fin n} (hij : i < j) (a : Fin n) :
+    a ∈ (singleton hij).signFinset i j ↔ i < a ∧ a < j := by
+  simp [signFinset]
+  intro h1 h2
+  rw [@singleton_getDual?_eq_none_iff_neq]
+  apply Or.inl
+  omega
+
+lemma subContraction_singleton_eq_singleton {φs : List 𝓕.States}
+    (φsΛ : WickContraction φs.length)
+    (a : φsΛ.1) : φsΛ.subContraction {a.1} (by simp) =
+    singleton (φsΛ.fstFieldOfContract_lt_sndFieldOfContract a) := by
+  apply Subtype.ext
+  simp [subContraction, singleton]
+  exact finset_eq_fstFieldOfContract_sndFieldOfContract φsΛ a
+
+end WickContraction
