HepLean/PerturbationTheory/WickContraction/SubContraction.lean
@@ -1,0 +1,137 @@
+/-
+Copyright (c) 2025 Joseph Tooby-Smith. All rights reserved.
+Released under Apache 2.0 license as described in the file LICENSE.
+Authors: Joseph Tooby-Smith
+-/
+import HepLean.PerturbationTheory.WickContraction.TimeContract
+import HepLean.PerturbationTheory.WickContraction.StaticContract
+import HepLean.PerturbationTheory.Algebras.FieldOpAlgebra.TimeContraction
+/-!
+
+# Sub  contractions
+
+-/
+
+open FieldSpecification
+variable {𝓕 : FieldSpecification}
+
+namespace WickContraction
+variable {n : ℕ} {φs : List 𝓕.States} {φsΛ : WickContraction φs.length}
+open HepLean.List
+open FieldOpAlgebra
+
+def subContraction (S : Finset (Finset (Fin φs.length))) (ha : S ⊆ φsΛ.1) : WickContraction φs.length :=
+  ⟨S, by
+    intro i hi
+    exact φsΛ.2.1 i (ha hi),
+    by
+    intro i hi j hj
+    exact φsΛ.2.2 i (ha hi) j (ha hj)⟩
+
+lemma mem_of_mem_subContraction {S : Finset (Finset (Fin φs.length))} {hs : S ⊆ φsΛ.1}
+    {a : Finset (Fin φs.length)} (ha : a ∈ (φsΛ.subContraction S hs).1) : a ∈ φsΛ.1 := by
+  exact hs ha
+
+def quotContraction (S : Finset (Finset (Fin φs.length))) (ha : S ⊆ φsΛ.1) :
+    WickContraction [φsΛ.subContraction S ha]ᵘᶜ.length :=
+  ⟨Finset.filter (fun a => Finset.map uncontractedListEmd a ∈ φsΛ.1) Finset.univ,
+  by
+    intro a ha'
+    simp at ha'
+    simpa using  φsΛ.2.1 (Finset.map uncontractedListEmd a) ha'
+    , by
+  intro a ha b hb
+  simp at ha hb
+  by_cases hab : a = b
+  · simp [hab]
+  · simp [hab]
+    have hx := φsΛ.2.2 (Finset.map uncontractedListEmd a) ha (Finset.map uncontractedListEmd b) hb
+    simp_all⟩
+
+lemma mem_of_mem_quotContraction {S : Finset (Finset (Fin φs.length))} {hs : S ⊆ φsΛ.1}
+    {a : Finset (Fin [φsΛ.subContraction S hs]ᵘᶜ.length)}
+    (ha : a ∈ (quotContraction S hs).1) : Finset.map uncontractedListEmd a ∈ φsΛ.1 := by
+  simp [quotContraction] at ha
+  exact ha
+
+lemma mem_subContraction_or_quotContraction {S : Finset (Finset (Fin φs.length))} {hs : S ⊆ φsΛ.1}
+    {a : Finset (Fin φs.length)} (ha : a ∈ φsΛ.1) :
+    a ∈ (φsΛ.subContraction S hs).1 ∨
+    ∃ a', Finset.map uncontractedListEmd a' = a ∧ a' ∈ (quotContraction S hs).1 := by
+  by_cases h1 : a ∈ (φsΛ.subContraction S hs).1
+  · simp [h1]
+  simp [h1]
+  simp [subContraction] at h1
+  have h2 := φsΛ.2.1 a ha
+  rw [@Finset.card_eq_two] at h2
+  obtain ⟨i, j, hij, rfl⟩ := h2
+  have hi : i ∈ (φsΛ.subContraction S hs).uncontracted := by
+    rw [mem_uncontracted_iff_not_contracted]
+    intro p hp
+    have hp' : p ∈ φsΛ.1 := hs hp
+    have hp2 := φsΛ.2.2 p hp' {i, j} ha
+    simp [subContraction] at hp
+    rcases hp2 with hp2 | hp2
+    · simp_all
+    simp at hp2
+    exact hp2.1
+  have hj : j ∈ (φsΛ.subContraction S hs).uncontracted := by
+    rw [mem_uncontracted_iff_not_contracted]
+    intro p hp
+    have hp' : p ∈ φsΛ.1 := hs hp
+    have hp2 := φsΛ.2.2 p hp' {i, j} ha
+    simp [subContraction] at hp
+    rcases hp2 with hp2 | hp2
+    · simp_all
+    simp at hp2
+    exact hp2.2
+  obtain ⟨i, rfl⟩ := uncontractedListEmd_surjective_mem_uncontracted i hi
+  obtain ⟨j, rfl⟩ := uncontractedListEmd_surjective_mem_uncontracted j hj
+  use {i, j}
+  simp [quotContraction]
+  exact ha
+
+@[simp]
+lemma subContraction_uncontractedList_get {S : Finset (Finset (Fin φs.length))} {hs : S ⊆ φsΛ.1}
+    {a : Fin [subContraction S hs]ᵘᶜ.length} :
+    [subContraction S hs]ᵘᶜ[a] = φs[uncontractedListEmd a] := by
+  erw [← getElem_uncontractedListEmd]
+  rfl
+
+@[simp]
+lemma quotContraction_fstFieldOfContract_uncontractedListEmd {S : Finset (Finset (Fin φs.length))}
+    {hs : S ⊆ φsΛ.1} (a : (quotContraction S hs).1) :
+    uncontractedListEmd ((quotContraction S hs).fstFieldOfContract a) =
+    (φsΛ.fstFieldOfContract ⟨Finset.map uncontractedListEmd a.1, mem_of_mem_quotContraction a.2⟩) := by
+  symm
+  apply eq_fstFieldOfContract_of_mem _ _ _ (uncontractedListEmd ((quotContraction S hs).sndFieldOfContract a) )
+  · simp only [Finset.mem_map', fstFieldOfContract_mem]
+  · simp
+  · apply uncontractedListEmd_strictMono
+    exact fstFieldOfContract_lt_sndFieldOfContract (quotContraction S hs) a
+
+@[simp]
+lemma quotContraction_sndFieldOfContract_uncontractedListEmd {S : Finset (Finset (Fin φs.length))}
+    {hs : S ⊆ φsΛ.1} (a : (quotContraction S hs).1) :
+    uncontractedListEmd ((quotContraction S hs).sndFieldOfContract a) =
+    (φsΛ.sndFieldOfContract ⟨Finset.map uncontractedListEmd a.1, mem_of_mem_quotContraction a.2⟩) := by
+  symm
+  apply eq_sndFieldOfContract_of_mem _ _ (uncontractedListEmd ((quotContraction S hs).fstFieldOfContract a) )
+  · simp only [Finset.mem_map', fstFieldOfContract_mem]
+  · simp
+  · apply uncontractedListEmd_strictMono
+    exact fstFieldOfContract_lt_sndFieldOfContract (quotContraction S hs) a
+
+lemma quotContraction_gradingCompliant {S : Finset (Finset (Fin φs.length))} {hs : S ⊆ φsΛ.1}
+    (hsΛ : φsΛ.GradingCompliant) :
+    GradingCompliant [φsΛ.subContraction S hs]ᵘᶜ (quotContraction S hs) := by
+  simp [GradingCompliant]
+  intro a ha
+  have h1' := mem_of_mem_quotContraction ha
+  erw [subContraction_uncontractedList_get]
+  erw [subContraction_uncontractedList_get]
+  simp
+  apply hsΛ
+
+
+end WickContraction
